Improve `PredType` with predicate lists

LeanMqtt/Primitives/PredType/Basic.lean
@@ -1,23 +1,43 @@
+import Lean
 import LeanMqtt.Core.Codec
 
 namespace Mqtt
 open Mqtt
 
-/--
+/-!
   `PredType` is a generic primitive for fields that are only correct when a
   given predicate is true.
 -/
-abbrev PredType {α : Type} (p : α → Prop) : Type :=
-  { val : α // p val }
+structure Condition where
+  desc : String
+  p : Prop
+  dec : Decidable p
 
-def PredType.serialize {α : Type} [c : Codec α] {p : α → Prop} (v : PredType p) : List UInt8 :=
+instance (c : Condition) : Decidable c.p := c.dec
+
+abbrev AllHold {α : Type} (gen : α → List Condition) (v : α) : Prop :=
+  ∀ c ∈ gen v, c.p
+
+abbrev PredType {α : Type} (gen : α → List Condition) : Type :=
+  { val : α // AllHold gen val }
+
+theorem PredType.get_proof {α : Type} {gen : α → List Condition} (v : PredType gen)
+    (idx : Nat) (h_idx : idx < (gen v.val).length := by exact of_decide_eq_true rfl) :
+    ((gen v.val).get ⟨idx, h_idx⟩).p :=
+  v.property _ (List.get_mem ..)
+
+def PredType.serialize {α : Type} [c : Codec α] {gen : α → List Condition} (v : PredType gen) : List UInt8 :=
   @Codec.serialize α c v.val
 
-def PredType.parser {α : Type} [c : Codec α] (p : α → Prop) [DecidablePred p] : Parser (PredType p) := do
+def PredType.parser {α : Type} [c : Codec α] (gen : α → List Condition) : Parser (PredType gen) := do
   let val ← @Codec.parser α c
-  if h : p val then
+  if h : AllHold gen val then
     return ⟨val, h⟩
   else
     failure
+
+macro "ensure! " p:term : term =>
+  let desc := Lean.Syntax.mkStrLit (toString p.raw)
+  `( { desc := $desc, p := $p, dec := inferInstance } )
 
 end Mqtt
